let x = 1 + 2 in let y = x + 3 in x + y
(*x = 3, y = 3 + 3, x + y = 3 + 6 = 9*)


(*sum [1;2;3]*)
let rec sum lst = match lst with
    | [] - > 0
    | x :: xs -> x + sum xs 

(*1 + 0, 1+ 2 + 0, 1 + 2 + 3 + 0 = 6*)

let rec foldl(f: 'b -> 'a -> 'b)(accum: 'b)(lst: 'a ->list) : 'b = match lst with
    | [] - > accum
    | x :: xs -> foldl f (f accum x) xs

let suml xs = foldl (+) 0 xs 

(*
    suml (1::2::3::[])
    ->foldl (+) 0 (1::2::3::[])
    ->foldl (+) ((+)0 1) (2::3::[])
    ->foldl (+) 1 (2::3::[])
    ->foldl (+) ((+)1 2) (3::[])
    ->foldl (+) 3 (3::[])
    ->foldl (+) ((x) 3 3) []
    ->foldl (+) 6 []
*)

let sumr xs = foldr (+) xs 0
(*           
   sumr (1::2::3::[])
-> foldr (+) (1::2::3::[]) 0
-> (+) 1 (foldr (+) (2::3::[]) 0)
-> (+) 1 ((+) 2 (foldr (+) (3::[]) 0))
-> (+) 1 ((+) 2 ((+) 3 (foldr (+) [] 0)))
-> (+) 1 ((+) 2 ((+) 3 0))
-> (+) 1 ((+) 2 3)
-> (+) 1 5
-> 6
*)